<?xml version="1.0"?>
<rdf:RDF xmlns="https://cwrusdle.bitbucket.io/Ontology/currentVoltage#"
     xml:base="https://cwrusdle.bitbucket.io/Ontology/currentVoltage"
     xmlns:owl="http://www.w3.org/2002/07/owl#"
     xmlns:rdf="http://www.w3.org/1999/02/22-rdf-syntax-ns#"
     xmlns:xml="http://www.w3.org/XML/1998/namespace"
     xmlns:xsd="http://www.w3.org/2001/XMLSchema#"
     xmlns:rdfs="http://www.w3.org/2000/01/rdf-schema#"
     xmlns:schema="https://www.schema.org/">
    <owl:Ontology rdf:about="https://cwrusdle.bitbucket.io/Ontology/currentVoltage">
        <rdfs:comment>This is an ontology for the current-voltage data acquisition method.</rdfs:comment>
    </owl:Ontology>
    


    <!-- 
    ///////////////////////////////////////////////////////////////////////////////////////
    //
    // Classes
    //
    ///////////////////////////////////////////////////////////////////////////////////////
     -->

    


    <!-- https://cwrusdle.bitbucket.io/Ontology/currentVoltage#CurrentShortCircuit -->

    <owl:Class rdf:about="https://cwrusdle.bitbucket.io/Ontology/currentVoltage#CurrentShortCircuit">
        <rdfs:subClassOf rdf:resource="https://cwrusdle.bitbucket.io/Ontology/currentVoltage#performanceParameters"/>
    </owl:Class>
    


    <!-- https://cwrusdle.bitbucket.io/Ontology/currentVoltage#ProdSpecficiations -->

    <owl:Class rdf:about="https://cwrusdle.bitbucket.io/Ontology/currentVoltage#ProdSpecficiations">
        <rdfs:subClassOf rdf:resource="https://cwrusdle.bitbucket.io/Ontology/currentVoltage#equipmentType"/>
        <rdfs:comment xml:lang="en">A single specification for a product</rdfs:comment>
        <rdfs:label xml:lang="en">ProdSpecifications</rdfs:label>
    </owl:Class>
    


    <!-- https://cwrusdle.bitbucket.io/Ontology/currentVoltage#TempRefCell -->

    <owl:Class rdf:about="https://cwrusdle.bitbucket.io/Ontology/currentVoltage#TempRefCell">
        <rdfs:subClassOf rdf:resource="https://cwrusdle.bitbucket.io/Ontology/currentVoltage#measurementSettings"/>
        <rdfs:comment xml:lang="en">Temperature of a reference cell.</rdfs:comment>
        <rdfs:label xml:lang="en">TempRefCell</rdfs:label>
    </owl:Class>
    


    <!-- https://cwrusdle.bitbucket.io/Ontology/currentVoltage#VoltageOpenCircuit -->

    <owl:Class rdf:about="https://cwrusdle.bitbucket.io/Ontology/currentVoltage#VoltageOpenCircuit">
        <rdfs:subClassOf rdf:resource="https://cwrusdle.bitbucket.io/Ontology/currentVoltage#performanceParameters"/>
    </owl:Class>
    


    <!-- https://cwrusdle.bitbucket.io/Ontology/currentVoltage#analysis -->

    <owl:Class rdf:about="https://cwrusdle.bitbucket.io/Ontology/currentVoltage#analysis">
        <rdfs:subClassOf rdf:resource="https://cwrusdle.bitbucket.io/Ontology/currentVoltage#currentVoltage"/>
        <rdfs:comment xml:lang="en">The curve fitting and associated parameters created from the curve fitting.</rdfs:comment>
        <rdfs:label xml:lang="en">analysis</rdfs:label>
    </owl:Class>
    


    <!-- https://cwrusdle.bitbucket.io/Ontology/currentVoltage#analysisMethod -->

    <owl:Class rdf:about="https://cwrusdle.bitbucket.io/Ontology/currentVoltage#analysisMethod">
        <rdfs:subClassOf rdf:resource="https://cwrusdle.bitbucket.io/Ontology/currentVoltage#analysis"/>
        <rdfs:comment xml:lang="en">The curve fitting and analysis method used to create the current voltage curve.</rdfs:comment>
        <rdfs:label xml:lang="en">analysisMethod</rdfs:label>
    </owl:Class>
    


    <!-- https://cwrusdle.bitbucket.io/Ontology/currentVoltage#calibrationSettings -->

    <owl:Class rdf:about="https://cwrusdle.bitbucket.io/Ontology/currentVoltage#calibrationSettings">
        <rdfs:subClassOf rdf:resource="https://cwrusdle.bitbucket.io/Ontology/currentVoltage#measurementSettings"/>
        <rdfs:comment xml:lang="en">Unique settings of measurement equipment.&quot;</rdfs:comment>
        <rdfs:label xml:lang="en">calibrationSettings</rdfs:label>
    </owl:Class>
    


    <!-- https://cwrusdle.bitbucket.io/Ontology/currentVoltage#currentVoltage -->

    <owl:Class rdf:about="https://cwrusdle.bitbucket.io/Ontology/currentVoltage#currentVoltage">
        <rdfs:comment xml:lang="en">A measurement method based on the current-voltage plot of photovoltaic systems.</rdfs:comment>
        <rdfs:label xml:lang="en">currentVoltage</rdfs:label>
    </owl:Class>
    


    <!-- https://cwrusdle.bitbucket.io/Ontology/currentVoltage#curves -->

    <owl:Class rdf:about="https://cwrusdle.bitbucket.io/Ontology/currentVoltage#curves">
        <rdfs:subClassOf rdf:resource="https://cwrusdle.bitbucket.io/Ontology/currentVoltage#currentVoltage"/>
        <rdfs:comment xml:lang="en">The base current voltage data that is to be used in the currentVoltage measurement method.</rdfs:comment>
        <rdfs:label xml:lang="en">curves</rdfs:label>
    </owl:Class>
    


    <!-- https://cwrusdle.bitbucket.io/Ontology/currentVoltage#equipmentType -->

    <owl:Class rdf:about="https://cwrusdle.bitbucket.io/Ontology/currentVoltage#equipmentType">
        <rdfs:subClassOf rdf:resource="https://cwrusdle.bitbucket.io/Ontology/currentVoltage#currentVoltage"/>
        <rdfs:comment xml:lang="en">The equipment used for the current voltage measurement.</rdfs:comment>
        <rdfs:label xml:lang="en">equipmentType</rdfs:label>
    </owl:Class>
    


    <!-- https://cwrusdle.bitbucket.io/Ontology/currentVoltage#fillFactor -->

    <owl:Class rdf:about="https://cwrusdle.bitbucket.io/Ontology/currentVoltage#fillFactor">
        <rdfs:subClassOf rdf:resource="https://cwrusdle.bitbucket.io/Ontology/currentVoltage#performanceParameters"/>
        <rdfs:comment xml:lang="en">The ratio of the maximum power to the product of the short circuit current and open circuit voltage.</rdfs:comment>
        <rdfs:label xml:lang="en">fillFactor</rdfs:label>
    </owl:Class>
    


    <!-- https://cwrusdle.bitbucket.io/Ontology/currentVoltage#flashDuration -->

    <owl:Class rdf:about="https://cwrusdle.bitbucket.io/Ontology/currentVoltage#flashDuration">
        <rdfs:subClassOf rdf:resource="https://cwrusdle.bitbucket.io/Ontology/currentVoltage#measurementSettings"/>
        <rdfs:comment xml:lang="en">The amount of time for a flash during currentVoltage measurement.</rdfs:comment>
        <rdfs:label xml:lang="en">flashDuration</rdfs:label>
    </owl:Class>
    


    <!-- https://cwrusdle.bitbucket.io/Ontology/currentVoltage#irradiance -->

    <owl:Class rdf:about="https://cwrusdle.bitbucket.io/Ontology/currentVoltage#irradiance">
        <rdfs:subClassOf rdf:resource="https://cwrusdle.bitbucket.io/Ontology/currentVoltage#measurementSettings"/>
        <rdfs:comment xml:lang="en">Measurement setting describing the intensity of the light energy.</rdfs:comment>
        <rdfs:label xml:lang="en">irradiance</rdfs:label>
    </owl:Class>
    


    <!-- https://cwrusdle.bitbucket.io/Ontology/currentVoltage#manufacturer -->

    <owl:Class rdf:about="https://cwrusdle.bitbucket.io/Ontology/currentVoltage#manufacturer">
        <rdfs:subClassOf rdf:resource="https://cwrusdle.bitbucket.io/Ontology/currentVoltage#equipmentType"/>
        <rdfs:comment xml:lang="en">The manufacturer of the product.</rdfs:comment>
        <rdfs:label xml:lang="en">manufacturer</rdfs:label>
    </owl:Class>
    


    <!-- https://cwrusdle.bitbucket.io/Ontology/currentVoltage#maximumPowerPoint -->

    <owl:Class rdf:about="https://cwrusdle.bitbucket.io/Ontology/currentVoltage#maximumPowerPoint">
        <rdfs:subClassOf rdf:resource="https://cwrusdle.bitbucket.io/Ontology/currentVoltage#performanceParameters"/>
        <rdfs:comment xml:lang="en">The point on the power curve that has the highest power output, or the product of the voltage and current.</rdfs:comment>
        <rdfs:label xml:lang="en">maximumPowerPoint</rdfs:label>
    </owl:Class>
    


    <!-- https://cwrusdle.bitbucket.io/Ontology/currentVoltage#measurementSettings -->

    <owl:Class rdf:about="https://cwrusdle.bitbucket.io/Ontology/currentVoltage#measurementSettings">
        <rdfs:subClassOf rdf:resource="https://cwrusdle.bitbucket.io/Ontology/currentVoltage#currentVoltage"/>
        <rdfs:comment xml:lang="en">The settings for the equipment used to measure the current voltage.</rdfs:comment>
        <rdfs:label xml:lang="en">measurementSettings</rdfs:label>
    </owl:Class>
    


    <!-- https://cwrusdle.bitbucket.io/Ontology/currentVoltage#measurementTechnique -->

    <owl:Class rdf:about="https://cwrusdle.bitbucket.io/Ontology/currentVoltage#measurementTechnique">
        <rdfs:subClassOf rdf:resource="https://cwrusdle.bitbucket.io/Ontology/currentVoltage#currentVoltage"/>
        <rdfs:comment xml:lang="en">The technique used to measure the CurrentVoltage data. The value can be dark, illuminated, or pseudo.</rdfs:comment>
        <rdfs:label xml:lang="en">measurementTechnique</rdfs:label>
    </owl:Class>
    


    <!-- https://cwrusdle.bitbucket.io/Ontology/currentVoltage#model -->

    <owl:Class rdf:about="https://cwrusdle.bitbucket.io/Ontology/currentVoltage#model">
        <rdfs:subClassOf rdf:resource="https://cwrusdle.bitbucket.io/Ontology/currentVoltage#equipmentType"/>
        <rdfs:comment xml:lang="en">The model of the product.</rdfs:comment>
        <rdfs:label xml:lang="en">model</rdfs:label>
    </owl:Class>
    


    <!-- https://cwrusdle.bitbucket.io/Ontology/currentVoltage#performanceParameters -->

    <owl:Class rdf:about="https://cwrusdle.bitbucket.io/Ontology/currentVoltage#performanceParameters">
        <rdfs:subClassOf rdf:resource="https://cwrusdle.bitbucket.io/Ontology/currentVoltage#analysis"/>
        <rdfs:comment xml:lang="en">The extracted parameters from the current voltage measurement.</rdfs:comment>
        <rdfs:label xml:lang="en">performanceParameters</rdfs:label>
    </owl:Class>
    


    <!-- https://cwrusdle.bitbucket.io/Ontology/currentVoltage#polarity -->

    <owl:Class rdf:about="https://cwrusdle.bitbucket.io/Ontology/currentVoltage#polarity">
        <rdfs:subClassOf rdf:resource="https://cwrusdle.bitbucket.io/Ontology/currentVoltage#measurementSettings"/>
        <rdfs:comment xml:lang="en">Positive or negative polarity for the voltage.</rdfs:comment>
        <rdfs:label xml:lang="en">polarity</rdfs:label>
    </owl:Class>
    


    <!-- https://cwrusdle.bitbucket.io/Ontology/currentVoltage#seriesResistance -->

    <owl:Class rdf:about="https://cwrusdle.bitbucket.io/Ontology/currentVoltage#seriesResistance">
        <rdfs:subClassOf rdf:resource="https://cwrusdle.bitbucket.io/Ontology/currentVoltage#performanceParameters"/>
        <rdfs:comment xml:lang="en">Equivalent resistance throughout the solar cell.</rdfs:comment>
        <rdfs:label xml:lang="en">seriesResistance</rdfs:label>
    </owl:Class>
    


    <!-- https://cwrusdle.bitbucket.io/Ontology/currentVoltage#shuntResistance -->

    <owl:Class rdf:about="https://cwrusdle.bitbucket.io/Ontology/currentVoltage#shuntResistance">
        <rdfs:subClassOf rdf:resource="https://cwrusdle.bitbucket.io/Ontology/currentVoltage#performanceParameters"/>
        <rdfs:comment xml:lang="en">The slope of the dark current versus applied voltage.</rdfs:comment>
        <rdfs:label xml:lang="en">shuntResistance</rdfs:label>
    </owl:Class>
    


    <!-- https://cwrusdle.bitbucket.io/Ontology/currentVoltage#spacialUniformity -->

    <owl:Class rdf:about="https://cwrusdle.bitbucket.io/Ontology/currentVoltage#spacialUniformity">
        <rdfs:subClassOf rdf:resource="https://cwrusdle.bitbucket.io/Ontology/currentVoltage#ProdSpecficiations"/>
        <rdfs:comment xml:lang="en">The measurement of how the irradiance varies over a defined area.</rdfs:comment>
        <rdfs:label xml:lang="en">spacialUniformity</rdfs:label>
    </owl:Class>
    


    <!-- https://cwrusdle.bitbucket.io/Ontology/currentVoltage#spectralClass -->

    <owl:Class rdf:about="https://cwrusdle.bitbucket.io/Ontology/currentVoltage#spectralClass">
        <rdfs:subClassOf rdf:resource="https://cwrusdle.bitbucket.io/Ontology/currentVoltage#ProdSpecficiations"/>
        <rdfs:comment xml:lang="en">Definition of how well the distribution of irradiance among different wavelengths approximates natural sunlight.</rdfs:comment>
        <rdfs:label xml:lang="en">spectralClass</rdfs:label>
    </owl:Class>
    


    <!-- https://cwrusdle.bitbucket.io/Ontology/currentVoltage#sweepType -->

    <owl:Class rdf:about="https://cwrusdle.bitbucket.io/Ontology/currentVoltage#sweepType">
        <rdfs:subClassOf rdf:resource="https://cwrusdle.bitbucket.io/Ontology/currentVoltage#measurementSettings"/>
        <rdfs:comment xml:lang="en">The sweep method used for current voltage measurement.</rdfs:comment>
        <rdfs:label xml:lang="en">sweepType</rdfs:label>
    </owl:Class>
    


    <!-- https://cwrusdle.bitbucket.io/Ontology/currentVoltage#temporalStability -->

    <owl:Class rdf:about="https://cwrusdle.bitbucket.io/Ontology/currentVoltage#temporalStability">
        <rdfs:subClassOf rdf:resource="https://cwrusdle.bitbucket.io/Ontology/currentVoltage#ProdSpecficiations"/>
        <rdfs:comment xml:lang="en">The output of a solar system at a certain spot, comparing the max irradiance and minimum irradiance.&quot;</rdfs:comment>
        <rdfs:label xml:lang="en">temporalStability</rdfs:label>
    </owl:Class>
    


    <!-- https://cwrusdle.bitbucket.io/Ontology/currentVoltage#timeStamp -->

    <owl:Class rdf:about="https://cwrusdle.bitbucket.io/Ontology/currentVoltage#timeStamp">
        <rdfs:subClassOf rdf:resource="https://cwrusdle.bitbucket.io/Ontology/currentVoltage#measurementSettings"/>
        <rdfs:comment xml:lang="en">The time at which the specific current voltage measurement took place.</rdfs:comment>
        <rdfs:label xml:lang="en">timeStamp</rdfs:label>
    </owl:Class>
</rdf:RDF>



<!-- Generated by the OWL API (version 4.5.9.2019-02-01T07:24:44Z) https://github.com/owlcs/owlapi -->

